\message{ !name(malament-solutions.tex)}\documentclass[12pt,fleqn]{article}
\setlength{\parskip}{1em}
\setlength{\parindent}{0em}
\usepackage{tensor}
\begin{document}

\message{ !name(malament-solutions.tex) !offset(-3) }


\[
  \begin{array}{lll} L_{\xi}(\tensor{\eta}{^a}\tensor{\eta}{^b})
    & = \eta ^aL_{\xi}(\eta ^b)+\eta ^bL_{\xi}(\eta ^a) \\
    & = \eta ^a\tensor{\delta}{^b_a}L_{\xi}(\eta ^a)+\eta ^bL_{\xi}(\eta ^a) \\
    & = \eta ^bL_{\xi}(\eta ^a)+\eta ^bL_{\xi}(\eta ^a) .\end{array}
\]

Thus, if $L_\xi (\eta ^a\eta ^b)=0$ then $\eta ^bL_\xi (\eta ^a)=0$.

\end{document} 
%%% Local Variables:
%%% mode: latex
%%% TeX-master: t
%%% End:

\message{ !name(malament-solutions.tex) !offset(-25) }
