\documentclass[12pt,fleqn]{article}
\usepackage{amsmath,amssymb}
\usepackage[letterpaper,left=1.25in,right=1.25in,top=1.2in,bottom=1.2in]{geometry}
\usepackage{array,enumitem}

\begin{document}

\vspace*{-4em}

\section*{Practice Problems: Predicate Logic}

\thispagestyle{empty}

\subsection*{A. Proofs}

\begin{enumerate}[leftmargin=*]

\item $Fa\:\vdash \: \forall x((a=x)\to Fx)$

  \begin{tabular}{r >{\centering\arraybackslash}p{1.0cm} p{6cm} >{\raggedright\arraybackslash}p{3.5cm}}
1 & (1) & $Fa$ & A \\
2 & (2) & $a = b$ & A \\
1,2 & (3) & $Fb$ & 1,2 =E \\
1 & (4) & $a = b \to Fb$ & 2,3 CP \\
1 & (5) & $\forall x (a = x \to Fx)$ & 4 UI \\
\end{tabular}

  
  

  \item $\vdash \:\forall x\forall y\bigl((Fx \wedge \neg Fy)
    \rightarrow x \neq y\bigr)$

  \begin{tabular}{r >{\centering\arraybackslash}p{1.0cm} p{7cm} >{\raggedright\arraybackslash}p{3.5cm}}
1 & (1) & $Fa \wedge \neg Fb$ & A \\
2 & (2) & $a = b$ & A \\
1 & (3) & $Fa$ & 1 $\wedge$E \\
1 & (4) & $\neg Fb$ & 1 $\wedge$E \\
1,2 & (5) & $Fb$ & 3,2 =E \\
1,2 & (6) & $Fb \wedge \neg Fb$ & 5,4 $\wedge$I \\
1 & (7) & $a\neq b$ & 2,6 RA \\
$\varnothing$ & (8) & $(Fa \wedge \neg Fb) \to a\neq b$ & 1,7 CP \\
$\varnothing$ & (9) & $\forall y ((Fa \wedge \neg Fy) \to a\neq y)$ & 8 UI \\
$\varnothing$ & (10) & $\forall x \forall y ((Fx \wedge \neg Fy) \to
                       x\neq y)$ & 9 UI \\
\end{tabular}
  

  \item $\forall x(Fx \rightarrow \exists y(Gy \wedge x = y)) \:\vdash\: \forall x(Fx \rightarrow Gx)$

  \item $\forall y(Ray \rightarrow y = b) \:\vdash\: \exists y(Ray \wedge Gy) \rightarrow Gb$

  \item $\forall x\forall y\forall z(Rxy \rightarrow \neg Ryz) \:\vdash\: \exists y\forall x\neg Rxy$

    First strategy: Assume the negation of the conclusion for RA. Use
    QN

  \begin{tabular}{r >{\centering\arraybackslash}p{1.0cm} p{7cm} >{\raggedright\arraybackslash}p{3.5cm}}
1 & (1) & $\forall x \forall y \forall z (Rxy \to \neg Ryz)$ & A \\
2 & (2) & $\neg \exists y \forall x \neg Rxy$ & A \\
2 & (3) & $\forall y \neg \forall x \neg Rxy$ & 2 QN \\
2 & (4) & $\neg \forall x \neg Rxb$ & 3 UE \\
2 & (5) & $\exists x \neg \neg Rxb$ & 4 QN \\
6 & (6) & $\neg \neg Rab$ & A \\
6 & (7) & $Rab$ & 6 DN \\
1 & (8) & $\forall y \forall z (Ray \to \neg Ryz)$ & 1 UE \\
1 & (9) & $\forall z (Rab \to \neg Rbz)$ & 8 UE \\
1 & (10) & $Rab \to \neg Rbc$ & 9 UE \\
1,6 & (11) & $\neg Rbc$ & 10,7 MP \\
1,2 & (12) & $\neg Rbc$ & 5,6,11 EE \\
1,2 & (13) & $\forall x \neg Rxc$ & 12 UI \\
1,2 & (14) & $\exists y \forall x \neg Rxy$ & 13 EI \\
1,2 & (15) & $\exists y \forall x \neg Rxy \wedge \neg \exists y \forall x \neg Rxy$ & 14,2 $\wedge$I \\
1 & (16) & $\neg \neg \exists y \forall x \neg Rxy$ & 2,15 RA \\
1 & (17) & $\exists y \forall x \neg Rxy$ & 16 DN \\
  \end{tabular}

  Second strategy: Either there is a pair of elements with an arrow
  between them or not. In the first case, there cannot be an arrow
  into the first element. In the second case, pick anything in the
  domain, and there is no arrow into it. In either case, there is
  something that has no arrow into it.

\begin{tabular}{r >{\centering\arraybackslash}p{1.0cm} p{7cm} >{\raggedright\arraybackslash}p{3.5cm}}
1 & (1) & $\forall x \forall y \forall z (Rxy \to \neg Ryz)$ & A \\
$\varnothing$ & (2) & $\exists y \exists x Rxy \vee \neg \exists y \exists x Rxy$ & prop taut \\
3 & (3) & $\exists y \exists x Rxy$ & A \\
4 & (4) & $\exists x Rxb$ & A \\
5 & (5) & $Rab$ & A \\
6 & (6) & $Rca$ & A \\
1 & (7) & $\forall y \forall z (Rcy \to \neg Ryz)$ & 1 UE \\
1 & (8) & $\forall z (Rca \to \neg Raz)$ & 7 UE \\
1 & (9) & $Rca \to \neg Rab$ & 8 UE \\
5 & (10) & $\neg \neg Rab$ & 5 DN \\
1,5 & (11) & $\neg Rca$ & 9,10 MT \\
1,5 & (12) & $\forall x \neg Rxa$ & 11 UI \\
1,5 & (13) & $\exists y \forall x \neg Rxy$ & 12 EI \\
1,4 & (14) & $\exists y \forall x \neg Rxy$ & 4,5,13 EE \\
1,3 & (15) & $\exists y \forall x \neg Rxy$ & 3,4,14 EE \\
16 & (16) & $\neg \exists y \exists x Rxy$ & A \\
16 & (17) & $\forall y \neg \exists x Rxy$ & 16 QN \\
16 & (18) & $\neg \exists x Rxa$ & 17 UE \\
16 & (19) & $\forall x \neg Rxa$ & 18 QN \\
16 & (20) & $\exists y \forall x \neg Rxy$ & 19 EI \\
1 & (21) & $\exists y \forall x \neg Rxy$ & 2,3,15,16,20 $\vee$E \\
\end{tabular}

    
  

  \item $\forall xFx \leftrightarrow \neg \exists x\exists y Rxy
    \:\vdash\: \exists x\forall y\forall z (Fx \rightarrow \neg Ryz)$

    First strategy: Either $\forall xFx$ or $\exists x\neg Fx$. In the
    former case, the premise gives $\neg\exists x\exists yRxy$, and QN
    gives $\forall y\forall z\neg Ryz$. In the latter case,
    $Fa\to \neg Rbc$ by negative paradox.

  \item $\vdash\: \forall x\exists y\forall z (\exists uTxyu
    \rightarrow \exists vTxzv )$

    We show how to derive the instance
    $\exists y\forall z(\exists uTayu\to \exists vTazv)$.  Up to
    $\alpha$-equivalence, the embedded conditional is of the form
    $\varphi (y)\to \varphi (z)$. So it's enough to prove that
    $\exists y\forall z(\varphi (y)\to \varphi (z))$. We have seen
    this before: it's a substitution instance of
    $\exists x\forall y(Fx\to Fy)$.
    

  \item Show that the sentence
    $\forall x\exists y\forall z(Rxy\wedge \neg Ryz)$ is inconsistent.

\begin{tabular}{>{\raggedleft\arraybackslash}p{1.5cm} >{\centering\arraybackslash}p{1.0cm} p{5cm} >{\raggedright\arraybackslash}p{3.5cm}}
1 & (1) & $\forall x \exists y \forall z (Rxy \wedge \neg Ryz)$ & A \\
1 & (2) & $\exists y \forall z (Ray \wedge \neg Ryz)$ & 1 UE \\
3 & (3) & $\forall z (Rab \wedge \neg Rbz)$ & A \\
1 & (4) & $\exists y \forall z (Rby \wedge \neg Ryz)$ & 1 UE \\
5 & (5) & $\forall z (Rbc \wedge \neg Rcz)$ & A \\
3 & (6) & $Rab \wedge \neg Rbc$ & 3 UE \\
5 & (7) & $Rbc \wedge \neg Rcd$ & 5 UE \\
3 & (8) & $\neg Rbc$ & 6 $\wedge$E \\
5 & (9) & $Rbc$ & 7 $\wedge$E \\
3,5 & (10) & $Rbc \wedge \neg Rbc$ & 9,8 $\wedge$I \\
3,5 & (11) & $P \wedge \neg P$ & 10 prop taut \\
1,3 & (12) & $P \wedge \neg P$ & 4,5,11 EE \\
1 & (13) & $P \wedge \neg P$ & 2,3,12 EE \\
\end{tabular}


\end{enumerate}

\end{document}
%%% Local Variables:
%%% mode: latex
%%% TeX-master: t
%%% End:
